<?xml version="1.0"?>
<rdf:RDF xmlns="https://w3id.org/EVI#"
     xml:base="https://w3id.org/EVI"
     xmlns:evi="https://w3id.org/EVI"
     xmlns:owl="http://www.w3.org/2002/07/owl#"
     xmlns:rdf="http://www.w3.org/1999/02/22-rdf-syntax-ns#"
     xmlns:xml="http://www.w3.org/XML/1998/namespace"
     xmlns:xsd="http://www.w3.org/2001/XMLSchema#"
     xmlns:rdfs="http://www.w3.org/2000/01/rdf-schema#"
     xmlns:swrl="http://www.w3.org/2003/11/swrl#"
     xmlns:vann="http://purl.org/vocab/vann/"
     xmlns:swrla="http://swrl.stanford.edu/ontologies/3.3/swrla.owl#"
     xmlns:swrlb="http://www.w3.org/2003/11/swrlb#"
     xmlns:terms="http://purl.org/dc/terms/">
    <owl:Ontology rdf:about="https://w3id.org/EVI">
        <terms:contributor>https://github.com/jniestroy</terms:contributor>
        <terms:contributor>https://github.com/mlev71</terms:contributor>
        <terms:created xml:lang="en">2020-07-27</terms:created>
        <terms:creator>https://datascience.virginia.edu/people/tim-clark</terms:creator>
        <terms:creator>https://github.com/sadnanalmanir</terms:creator>
        <terms:description xml:lang="en">The Evidence Graph ontology extends core concepts from the W3C Provenance Ontology PROV-O and Bioschemas&apos; Profiles to describe evidence for correctness of findings in biomedical publications. The semantic data model in EVI is expressed using OWL2 Web Ontology Language (OWL2).</terms:description>
        <terms:license>http://creativecommons.org/licenses/by-nc-sa/2.0/</terms:license>
        <terms:title xml:lang="en">EVI: Evidence Graph Ontology</terms:title>
        <vann:preferredNamespacePrefix>evi</vann:preferredNamespacePrefix>
        <vann:preferredNamespaceUri xml:lang="en">http://w3id.org/evi/</vann:preferredNamespaceUri>
        <owl:versionIRI xml:lang="en">http://www.w3.org/2002/07/owl</owl:versionIRI>
        <owl:versionInfo xml:lang="en">0.1</owl:versionInfo>
    </owl:Ontology>
    


    <!-- 
    ///////////////////////////////////////////////////////////////////////////////////////
    //
    // Annotation properties
    //
    ///////////////////////////////////////////////////////////////////////////////////////
     -->

    


    <!-- http://purl.org/dc/terms/contributor -->

    <owl:AnnotationProperty rdf:about="http://purl.org/dc/terms/contributor"/>
    


    <!-- http://purl.org/dc/terms/created -->

    <owl:AnnotationProperty rdf:about="http://purl.org/dc/terms/created"/>
    


    <!-- http://purl.org/dc/terms/creator -->

    <owl:AnnotationProperty rdf:about="http://purl.org/dc/terms/creator"/>
    


    <!-- http://purl.org/dc/terms/description -->

    <owl:AnnotationProperty rdf:about="http://purl.org/dc/terms/description"/>
    


    <!-- http://purl.org/dc/terms/license -->

    <owl:AnnotationProperty rdf:about="http://purl.org/dc/terms/license"/>
    


    <!-- http://purl.org/dc/terms/title -->

    <owl:AnnotationProperty rdf:about="http://purl.org/dc/terms/title"/>
    


    <!-- http://purl.org/vocab/vann/preferredNamespacePrefix -->

    <owl:AnnotationProperty rdf:about="http://purl.org/vocab/vann/preferredNamespacePrefix"/>
    


    <!-- http://purl.org/vocab/vann/preferredNamespaceUri -->

    <owl:AnnotationProperty rdf:about="http://purl.org/vocab/vann/preferredNamespaceUri"/>
    


    <!-- http://swrl.stanford.edu/ontologies/3.3/swrla.owl#isRuleEnabled -->

    <owl:AnnotationProperty rdf:about="http://swrl.stanford.edu/ontologies/3.3/swrla.owl#isRuleEnabled"/>
    


    <!-- http://www.w3.org/2002/07/owl#versionIRI -->

    <owl:AnnotationProperty rdf:about="http://www.w3.org/2002/07/owl#versionIRI"/>
    


    <!-- 
    ///////////////////////////////////////////////////////////////////////////////////////
    //
    // Object Properties
    //
    ///////////////////////////////////////////////////////////////////////////////////////
     -->

    


    <!-- https://w3id.org/EVI#about -->

    <owl:ObjectProperty rdf:about="https://w3id.org/EVI#about">
        <rdfs:domain rdf:resource="https://w3id.org/EVI#Caption"/>
        <rdfs:range rdf:resource="http://schema.org/Dataset"/>
        <rdfs:comment>Asserts instance of a Caption about a Dataset.</rdfs:comment>
        <rdfs:label>about</rdfs:label>
    </owl:ObjectProperty>
    


    <!-- https://w3id.org/EVI#arguedBy -->

    <owl:ObjectProperty rdf:about="https://w3id.org/EVI#arguedBy">
        <owl:inverseOf rdf:resource="https://w3id.org/EVI#argues"/>
        <rdfs:comment>Asserts that the principal Claim is arguedBy an EvideneGraph.</rdfs:comment>
        <rdfs:label>arguedBy</rdfs:label>
    </owl:ObjectProperty>
    


    <!-- https://w3id.org/EVI#argues -->

    <owl:ObjectProperty rdf:about="https://w3id.org/EVI#argues">
        <rdfs:domain rdf:resource="https://w3id.org/EVI#EvidenceGraph"/>
        <rdfs:range rdf:resource="http://schema.org/Claim"/>
        <rdfs:comment>Asserts that EvidenceGraph argues the principal Claim.</rdfs:comment>
        <rdfs:label>argues</rdfs:label>
    </owl:ObjectProperty>
    


    <!-- https://w3id.org/EVI#assertedBy -->

    <owl:ObjectProperty rdf:about="https://w3id.org/EVI#assertedBy">
        <owl:inverseOf rdf:resource="https://w3id.org/EVI#asserts"/>
        <rdfs:comment>Instance of Representation assertedBy instance of EvidenceGraph.</rdfs:comment>
        <rdfs:label>assertedBy</rdfs:label>
    </owl:ObjectProperty>
    


    <!-- https://w3id.org/EVI#asserts -->

    <owl:ObjectProperty rdf:about="https://w3id.org/EVI#asserts">
        <rdfs:subPropertyOf rdf:resource="https://w3id.org/EVI#contains"/>
        <rdfs:domain rdf:resource="https://w3id.org/EVI#EvidenceGraph"/>
        <rdfs:range rdf:resource="https://w3id.org/EVI#Representation"/>
        <rdfs:comment>Instance of EvidenceGraph asserts instance of Representation.</rdfs:comment>
        <rdfs:label>asserts</rdfs:label>
    </owl:ObjectProperty>
    


    <!-- https://w3id.org/EVI#associatedWith -->

    <owl:ObjectProperty rdf:about="https://w3id.org/EVI#associatedWith">
        <rdfs:subPropertyOf rdf:resource="https://www.w3.org/ns/prov#wasAssociatedWith"/>
        <rdfs:domain rdf:resource="https://www.w3.org/ns/prov#Activity"/>
        <rdfs:range rdf:resource="https://www.w3.org/ns/prov#Agent"/>
        <rdfs:comment>A prov:Agent that had some (unspecified) responsibility for the occurrence of this prov:Activity.</rdfs:comment>
        <rdfs:label>associatedWith</rdfs:label>
    </owl:ObjectProperty>
    


    <!-- https://w3id.org/EVI#attributedTo -->

    <owl:ObjectProperty rdf:about="https://w3id.org/EVI#attributedTo">
        <rdfs:subPropertyOf rdf:resource="https://www.w3.org/ns/prov#wasAttributedTo"/>
        <rdfs:domain rdf:resource="https://www.w3.org/ns/prov#Entity"/>
        <rdfs:range rdf:resource="https://www.w3.org/ns/prov#Agent"/>
        <rdfs:comment>Attribution is the ascribing of a prov:Entity to a prov:Agent.</rdfs:comment>
        <rdfs:label>attributedTo</rdfs:label>
    </owl:ObjectProperty>
    


    <!-- https://w3id.org/EVI#challengedBy -->

    <owl:ObjectProperty rdf:about="https://w3id.org/EVI#challengedBy">
        <owl:inverseOf rdf:resource="https://w3id.org/EVI#challenges"/>
        <rdfs:comment>Reverse of challenges property.</rdfs:comment>
        <rdfs:label>challengedBy</rdfs:label>
    </owl:ObjectProperty>
    


    <!-- https://w3id.org/EVI#challenges -->

    <owl:ObjectProperty rdf:about="https://w3id.org/EVI#challenges">
        <rdfs:domain rdf:resource="https://w3id.org/EVI#Representation"/>
        <rdfs:range rdf:resource="https://w3id.org/EVI#Representation"/>
        <rdfs:comment>The challenges property is inferred when Representation either directlyChallenges another, or indirectlyChallenges it by undercutting (directlyChallenges) a Representation which supports it.</rdfs:comment>
        <rdfs:label>challenges</rdfs:label>
    </owl:ObjectProperty>
    


    <!-- https://w3id.org/EVI#contains -->

    <owl:ObjectProperty rdf:about="https://w3id.org/EVI#contains">
        <rdfs:domain rdf:resource="https://w3id.org/EVI#Representation"/>
        <rdfs:range rdf:resource="https://w3id.org/EVI#Representation"/>
        <rdfs:comment>Instances of Representations may contain instances of  Representations.</rdfs:comment>
        <rdfs:label>contains</rdfs:label>
    </owl:ObjectProperty>
    


    <!-- https://w3id.org/EVI#creator -->

    <owl:ObjectProperty rdf:about="https://w3id.org/EVI#creator">
        <rdfs:domain rdf:resource="https://w3id.org/EVI#Representation"/>
        <rdfs:range rdf:resource="https://www.w3.org/ns/prov#Agent"/>
        <rdfs:comment>An instance of Representation responsible for making the resource. Recommended practice is to identify the creator with a URI.</rdfs:comment>
        <rdfs:label>creator</rdfs:label>
    </owl:ObjectProperty>
    


    <!-- https://w3id.org/EVI#derivedFrom -->

    <owl:ObjectProperty rdf:about="https://w3id.org/EVI#derivedFrom">
        <rdfs:subPropertyOf rdf:resource="https://www.w3.org/ns/prov#wasDerivedFrom"/>
        <rdfs:domain rdf:resource="https://www.w3.org/ns/prov#Entity"/>
        <rdfs:range rdf:resource="https://www.w3.org/ns/prov#Entity"/>
        <rdfs:comment>A derivation is a transformation of a prov:Entity into another, an update of a prov:Entity resulting in a new one, or the construction of a new prov:Entity based on a pre-existing prov:Entity.</rdfs:comment>
        <rdfs:label>derivedFrom</rdfs:label>
    </owl:ObjectProperty>
    


    <!-- https://w3id.org/EVI#directlyChallengedBy -->

    <owl:ObjectProperty rdf:about="https://w3id.org/EVI#directlyChallengedBy">
        <rdfs:subPropertyOf rdf:resource="https://w3id.org/EVI#challengedBy"/>
        <owl:inverseOf rdf:resource="https://w3id.org/EVI#directlyChallenges"/>
        <rdfs:comment>Reverse of directlyChallenges property.</rdfs:comment>
        <rdfs:label>directlyChallengedBy</rdfs:label>
    </owl:ObjectProperty>
    


    <!-- https://w3id.org/EVI#directlyChallenges -->

    <owl:ObjectProperty rdf:about="https://w3id.org/EVI#directlyChallenges">
        <rdfs:subPropertyOf rdf:resource="https://w3id.org/EVI#challenges"/>
        <rdfs:comment>The directlyChallenges property establishes a relation between instances of Representations when they directly challenge one another.</rdfs:comment>
        <rdfs:label>directlyChallenges</rdfs:label>
    </owl:ObjectProperty>
    


    <!-- https://w3id.org/EVI#directlySupportedBy -->

    <owl:ObjectProperty rdf:about="https://w3id.org/EVI#directlySupportedBy">
        <rdfs:subPropertyOf rdf:resource="https://w3id.org/EVI#supportedBy"/>
        <owl:inverseOf rdf:resource="https://w3id.org/EVI#directlySupports"/>
        <rdfs:comment>The use of directlySupportedBy property is intended to establish a direct relation between instances of  Representations.</rdfs:comment>
        <rdfs:label>directlySupportedBy</rdfs:label>
    </owl:ObjectProperty>
    


    <!-- https://w3id.org/EVI#directlySupports -->

    <owl:ObjectProperty rdf:about="https://w3id.org/EVI#directlySupports">
        <rdfs:subPropertyOf rdf:resource="https://w3id.org/EVI#supports"/>
        <rdfs:comment>The use of directlySupports property is intended to establish a direct relation between instances of  Representations.</rdfs:comment>
        <rdfs:label>directlySupports</rdfs:label>
    </owl:ObjectProperty>
    


    <!-- https://w3id.org/EVI#generatedBy -->

    <owl:ObjectProperty rdf:about="https://w3id.org/EVI#generatedBy">
        <rdfs:subPropertyOf rdf:resource="https://www.w3.org/ns/prov#wasGeneratedBy"/>
        <rdfs:domain rdf:resource="https://www.w3.org/ns/prov#Entity"/>
        <rdfs:range rdf:resource="https://www.w3.org/ns/prov#Activity"/>
        <rdfs:comment>Generation is the completion of production of a new entity by an activity. This entity did not exist before generation and becomes available for usage after this generation.</rdfs:comment>
        <rdfs:label>generatedBy</rdfs:label>
    </owl:ObjectProperty>
    


    <!-- https://w3id.org/EVI#indirectlyChallengedBy -->

    <owl:ObjectProperty rdf:about="https://w3id.org/EVI#indirectlyChallengedBy">
        <rdfs:subPropertyOf rdf:resource="https://w3id.org/EVI#challengedBy"/>
        <owl:inverseOf rdf:resource="https://w3id.org/EVI#indirectlyChallenges"/>
        <rdfs:comment>Reverse of indirectlyChallenges property.</rdfs:comment>
        <rdfs:label>indirectlyChallengedBy</rdfs:label>
    </owl:ObjectProperty>
    


    <!-- https://w3id.org/EVI#indirectlyChallenges -->

    <owl:ObjectProperty rdf:about="https://w3id.org/EVI#indirectlyChallenges">
        <rdfs:subPropertyOf rdf:resource="https://w3id.org/EVI#challenges"/>
        <owl:propertyChainAxiom rdf:parseType="Collection">
            <rdf:Description rdf:about="https://w3id.org/EVI#directlyChallenges"/>
            <rdf:Description rdf:about="https://w3id.org/EVI#supports"/>
        </owl:propertyChainAxiom>
        <rdfs:comment>The indirectlyChallenges property establishes a relation between instances of Representations when they indirectly challenge one another with the help of property chaining.</rdfs:comment>
        <rdfs:label>indirectlyChallenges</rdfs:label>
    </owl:ObjectProperty>
    


    <!-- https://w3id.org/EVI#representedBy -->

    <owl:ObjectProperty rdf:about="https://w3id.org/EVI#representedBy">
        <owl:inverseOf rdf:resource="https://w3id.org/EVI#represents"/>
        <rdfs:comment>Instances of prov:Entity may be represented by instance of Representation.</rdfs:comment>
        <rdfs:label>representedBy</rdfs:label>
    </owl:ObjectProperty>
    


    <!-- https://w3id.org/EVI#represents -->

    <owl:ObjectProperty rdf:about="https://w3id.org/EVI#represents">
        <rdfs:domain rdf:resource="https://w3id.org/EVI#Representation"/>
        <rdfs:range rdf:resource="https://www.w3.org/ns/prov#Entity"/>
        <rdfs:comment>Instance of Representation may represent instance of prov:Entity.</rdfs:comment>
        <rdfs:label>represents</rdfs:label>
    </owl:ObjectProperty>
    


    <!-- https://w3id.org/EVI#supportedBy -->

    <owl:ObjectProperty rdf:about="https://w3id.org/EVI#supportedBy">
        <owl:inverseOf rdf:resource="https://w3id.org/EVI#supports"/>
        <rdfs:comment>The supportedBy property is a transitive relation between Representations.</rdfs:comment>
        <rdfs:label>supportedBy</rdfs:label>
    </owl:ObjectProperty>
    


    <!-- https://w3id.org/EVI#supports -->

    <owl:ObjectProperty rdf:about="https://w3id.org/EVI#supports">
        <rdf:type rdf:resource="http://www.w3.org/2002/07/owl#TransitiveProperty"/>
        <rdfs:domain rdf:resource="https://w3id.org/EVI#Representation"/>
        <rdfs:range rdf:resource="https://w3id.org/EVI#Representation"/>
        <rdfs:comment>The supports property is a transitive relation between Representations.</rdfs:comment>
        <rdfs:label>supports</rdfs:label>
    </owl:ObjectProperty>
    


    <!-- https://w3id.org/EVI#used -->

    <owl:ObjectProperty rdf:about="https://w3id.org/EVI#used">
        <owl:inverseOf rdf:resource="https://w3id.org/EVI#usedBy"/>
        <rdfs:domain rdf:resource="https://www.w3.org/ns/prov#Activity"/>
        <rdfs:range rdf:resource="https://www.w3.org/ns/prov#Entity"/>
        <rdfs:comment>A prov:Activity that used a prov:Entity.</rdfs:comment>
        <rdfs:comment>The more specific usedDataset, usedService, usedSoftware properties should be used whenever possible.</rdfs:comment>
        <rdfs:label>used</rdfs:label>
    </owl:ObjectProperty>
    


    <!-- https://w3id.org/EVI#usedBy -->

    <owl:ObjectProperty rdf:about="https://w3id.org/EVI#usedBy">
        <rdfs:comment>A prov:Entity that was used by a prov:Activity.</rdfs:comment>
        <rdfs:label>usedBy</rdfs:label>
    </owl:ObjectProperty>
    


    <!-- https://w3id.org/EVI#usedDataset -->

    <owl:ObjectProperty rdf:about="https://w3id.org/EVI#usedDataset">
        <rdfs:subPropertyOf rdf:resource="https://w3id.org/EVI#used"/>
        <rdfs:domain rdf:resource="https://w3id.org/EVI#Computation"/>
        <rdfs:range rdf:resource="https://w3id.org/EVI#Dataset"/>
        <rdfs:comment>A Computation as a prov:Activity that used Dataset as a prov:Entity.</rdfs:comment>
        <rdfs:label>usedDataset</rdfs:label>
    </owl:ObjectProperty>
    


    <!-- https://w3id.org/EVI#usedService -->

    <owl:ObjectProperty rdf:about="https://w3id.org/EVI#usedService">
        <rdfs:subPropertyOf rdf:resource="https://w3id.org/EVI#used"/>
        <rdfs:domain rdf:resource="https://w3id.org/EVI#Computation"/>
        <rdfs:range rdf:resource="https://w3id.org/EVI#Service"/>
        <rdfs:comment>A Computation as a prov:Activity that used Service as a prov:Entity.</rdfs:comment>
        <rdfs:label>usedService</rdfs:label>
    </owl:ObjectProperty>
    


    <!-- https://w3id.org/EVI#usedSoftware -->

    <owl:ObjectProperty rdf:about="https://w3id.org/EVI#usedSoftware">
        <rdfs:subPropertyOf rdf:resource="https://w3id.org/EVI#used"/>
        <rdfs:domain rdf:resource="https://w3id.org/EVI#Computation"/>
        <rdfs:range rdf:resource="https://w3id.org/EVI#Software"/>
        <rdfs:comment>A Computation as a prov:Activity that used Software as a prov:Entity.</rdfs:comment>
        <rdfs:label>usedSoftware</rdfs:label>
    </owl:ObjectProperty>
    


    <!-- https://www.w3.org/ns/prov#wasAssociatedWith -->

    <owl:ObjectProperty rdf:about="https://www.w3.org/ns/prov#wasAssociatedWith">
        <rdfs:comment>A prov:Agent that had some (unspecified) responsibility for the occurrence of this prov:Activity.</rdfs:comment>
        <rdfs:comment>The more specific associatedWith property should be used whenever possible.</rdfs:comment>
        <rdfs:label>wasAssociatedWith</rdfs:label>
    </owl:ObjectProperty>
    


    <!-- https://www.w3.org/ns/prov#wasAttributedTo -->

    <owl:ObjectProperty rdf:about="https://www.w3.org/ns/prov#wasAttributedTo">
        <rdfs:comment>Attribution is the ascribing of a prov:Entity to a prov:Agent.</rdfs:comment>
        <rdfs:comment>The more specific attributedTo property should be used whenever possible.</rdfs:comment>
        <rdfs:label>wasAttributedTo</rdfs:label>
    </owl:ObjectProperty>
    


    <!-- https://www.w3.org/ns/prov#wasDerivedFrom -->

    <owl:ObjectProperty rdf:about="https://www.w3.org/ns/prov#wasDerivedFrom">
        <rdfs:comment>A derivation is a transformation of a prov:Entity into another, an update of a prov:Entity resulting in a new one, or the construction of a new prov:Entity based on a pre-existing prov:Entity.</rdfs:comment>
        <rdfs:comment>The more specific derivedFrom property should be used whenever possible.</rdfs:comment>
        <rdfs:label>wasDerivedFrom</rdfs:label>
    </owl:ObjectProperty>
    


    <!-- https://www.w3.org/ns/prov#wasGeneratedBy -->

    <owl:ObjectProperty rdf:about="https://www.w3.org/ns/prov#wasGeneratedBy">
        <rdfs:comment>Generation is the completion of production of a new entity by an activity. This entity did not exist before generation and becomes available for usage after this generation.</rdfs:comment>
        <rdfs:comment>The more specific generatedBy property should be used whenever possible.</rdfs:comment>
        <rdfs:label>wasGeneratedBy</rdfs:label>
    </owl:ObjectProperty>
    


    <!-- 
    ///////////////////////////////////////////////////////////////////////////////////////
    //
    // Data properties
    //
    ///////////////////////////////////////////////////////////////////////////////////////
     -->

    


    <!-- https://schema.org/contentUrl -->

    <owl:DatatypeProperty rdf:about="https://schema.org/contentUrl">
        <rdfs:range rdf:resource="http://www.w3.org/2001/XMLSchema#anyURI"/>
        <rdfs:comment>A URL for the media object in the form of xsd:anyURI.</rdfs:comment>
        <rdfs:comment>Actual bytes of the media object, for example the image file or video file</rdfs:comment>
        <rdfs:label>contentUrl</rdfs:label>
    </owl:DatatypeProperty>
    


    <!-- https://w3id.org/EVI#citation -->

    <owl:DatatypeProperty rdf:about="https://w3id.org/EVI#citation">
        <rdfs:domain rdf:resource="https://w3id.org/EVI#Reference"/>
        <rdfs:range rdf:resource="http://www.w3.org/2001/XMLSchema#string"/>
        <rdfs:comment>The description of Reference in the form of xsd:string.</rdfs:comment>
        <rdfs:label>citation</rdfs:label>
    </owl:DatatypeProperty>
    


    <!-- https://w3id.org/EVI#id -->

    <owl:DatatypeProperty rdf:about="https://w3id.org/EVI#id">
        <rdfs:comment>An identifier to specify an object.</rdfs:comment>
        <rdfs:label>id</rdfs:label>
    </owl:DatatypeProperty>
    


    <!-- https://w3id.org/EVI#state -->

    <owl:DatatypeProperty rdf:about="https://w3id.org/EVI#state">
        <rdfs:domain rdf:resource="https://w3id.org/EVI#Claim"/>
        <rdfs:range rdf:resource="http://www.w3.org/2001/XMLSchema#string"/>
        <rdfs:comment>The statement of Claim in the form of xsd:string.</rdfs:comment>
        <rdfs:label>state</rdfs:label>
    </owl:DatatypeProperty>
    


    <!-- https://www.w3.org/ns/prov#atTime -->

    <owl:DatatypeProperty rdf:about="https://www.w3.org/ns/prov#atTime">
        <rdfs:comment>The PROV data model is implicitly based on a notion of instantaneous events (or just events), that mark transitions in the world. Events include generation, usage, or invalidation of entities, as well as starting or ending of activities. This notion of event is not first-class in the data model, but it is useful for explaining its other concepts and its semantics.</rdfs:comment>
        <rdfs:label>atTime</rdfs:label>
    </owl:DatatypeProperty>
    


    <!-- 
    ///////////////////////////////////////////////////////////////////////////////////////
    //
    // Classes
    //
    ///////////////////////////////////////////////////////////////////////////////////////
     -->

    


    <!-- http://schema.org/Article -->

    <owl:Class rdf:about="http://schema.org/Article">
        <owl:equivalentClass rdf:resource="https://w3id.org/EVI#Article"/>
        <rdfs:subClassOf rdf:resource="https://w3id.org/EVI#Representation"/>
        <rdfs:comment>An identifiable source object of which an EvidenceGraph is derived. It includes information about its location, time of creation, and the authors.</rdfs:comment>
        <rdfs:label>Article</rdfs:label>
    </owl:Class>
    


    <!-- http://schema.org/Claim -->

    <owl:Class rdf:about="http://schema.org/Claim">
        <owl:equivalentClass rdf:resource="https://w3id.org/EVI#Claim"/>
        <rdfs:subClassOf rdf:resource="https://w3id.org/EVI#Representation"/>
        <rdfs:comment>A Claim is a principal statement arguedBy a EvidenceGraph in a scientific Article.</rdfs:comment>
        <rdfs:label>Claim</rdfs:label>
    </owl:Class>
    


    <!-- http://schema.org/Dataset -->

    <owl:Class rdf:about="http://schema.org/Dataset">
        <owl:equivalentClass rdf:resource="https://w3id.org/EVI#Dataset"/>
        <rdfs:subClassOf rdf:resource="https://w3id.org/EVI#Representation"/>
        <rdfs:comment>A body of structured information describing some topic(s) of interest.</rdfs:comment>
        <rdfs:label>Dataset</rdfs:label>
    </owl:Class>
    


    <!-- http://schema.org/Organization -->

    <owl:Class rdf:about="http://schema.org/Organization">
        <owl:equivalentClass rdf:resource="https://www.w3.org/ns/prov#Organization"/>
        <rdfs:subClassOf rdf:resource="https://www.w3.org/ns/prov#Agent"/>
        <rdfs:comment>An organization is a social or legal institution such as a company, society, etc.</rdfs:comment>
        <rdfs:label>Organization</rdfs:label>
    </owl:Class>
    


    <!-- http://schema.org/Person -->

    <owl:Class rdf:about="http://schema.org/Person">
        <owl:equivalentClass rdf:resource="https://www.w3.org/ns/prov#Person"/>
        <rdfs:subClassOf rdf:resource="https://www.w3.org/ns/prov#Agent"/>
        <rdfs:comment>Person agents are people.</rdfs:comment>
        <rdfs:label>Person</rdfs:label>
    </owl:Class>
    


    <!-- http://schema.org/Service -->

    <owl:Class rdf:about="http://schema.org/Service">
        <owl:equivalentClass rdf:resource="https://w3id.org/EVI#Service"/>
        <rdfs:subClassOf rdf:resource="https://w3id.org/EVI#Method"/>
        <rdfs:comment>A Method used during a Computation Activity.</rdfs:comment>
        <rdfs:label>Service</rdfs:label>
    </owl:Class>
    


    <!-- http://schema.org/SoftwareApplication -->

    <owl:Class rdf:about="http://schema.org/SoftwareApplication">
        <owl:equivalentClass rdf:resource="https://w3id.org/EVI#Software"/>
        <rdfs:subClassOf rdf:resource="https://w3id.org/EVI#Material"/>
        <rdfs:comment>A set of instructions to perform specific Computation Activity.</rdfs:comment>
        <rdfs:label>SoftwareApplication</rdfs:label>
    </owl:Class>
    


    <!-- https://w3id.org/EVI#Article -->

    <owl:Class rdf:about="https://w3id.org/EVI#Article">
        <rdfs:subClassOf rdf:resource="https://w3id.org/EVI#Representation"/>
        <rdfs:label>Article</rdfs:label>
    </owl:Class>
    


    <!-- https://w3id.org/EVI#Caption -->

    <owl:Class rdf:about="https://w3id.org/EVI#Caption">
        <rdfs:subClassOf rdf:resource="http://schema.org/Claim"/>
        <rdfs:comment>A composition of descriptive statements which describes information about objects such as images, tables, datasets etc.</rdfs:comment>
        <rdfs:label>Caption</rdfs:label>
    </owl:Class>
    


    <!-- https://w3id.org/EVI#Claim -->

    <owl:Class rdf:about="https://w3id.org/EVI#Claim">
        <rdfs:subClassOf rdf:resource="https://w3id.org/EVI#Representation"/>
        <rdfs:comment>A Claim is a principal statement arguedBy a EvidenceGraph in a scientific Article.</rdfs:comment>
        <rdfs:label>Claim</rdfs:label>
    </owl:Class>
    


    <!-- https://w3id.org/EVI#Computation -->

    <owl:Class rdf:about="https://w3id.org/EVI#Computation">
        <rdfs:subClassOf rdf:resource="https://www.w3.org/ns/prov#Activity"/>
        <rdfs:comment>Computation is an Activity which is generally performed on a Dataset with the help of a SoftwareApplication</rdfs:comment>
        <rdfs:label>Computation</rdfs:label>
    </owl:Class>
    


    <!-- https://w3id.org/EVI#Dataset -->

    <owl:Class rdf:about="https://w3id.org/EVI#Dataset">
        <rdfs:subClassOf rdf:resource="https://w3id.org/EVI#Representation"/>
        <rdfs:comment>A body of structured information describing some topic(s) of interest.</rdfs:comment>
        <rdfs:label>Dataset</rdfs:label>
    </owl:Class>
    


    <!-- https://w3id.org/EVI#EvidenceGraph -->

    <owl:Class rdf:about="https://w3id.org/EVI#EvidenceGraph">
        <rdfs:subClassOf rdf:resource="https://w3id.org/EVI#Representation"/>
        <rdfs:comment>An EvidenceGraph is a set of Representations, having supports and / or challenges relations to one another, and potentially those which have Reference to other EvidenceGraphs.</rdfs:comment>
        <rdfs:label>EvidenceGraph</rdfs:label>
    </owl:Class>
    


    <!-- https://w3id.org/EVI#Material -->

    <owl:Class rdf:about="https://w3id.org/EVI#Material">
        <rdfs:subClassOf rdf:resource="https://w3id.org/EVI#Representation"/>
        <rdfs:comment>A Material supports any Method of which it is a component.</rdfs:comment>
        <rdfs:label>Material</rdfs:label>
    </owl:Class>
    


    <!-- https://w3id.org/EVI#Method -->

    <owl:Class rdf:about="https://w3id.org/EVI#Method">
        <rdfs:subClassOf rdf:resource="https://w3id.org/EVI#Representation"/>
        <rdfs:comment>A reusable recipe showing how the Dataset were obtained. It specifies an Activitiy, and may refer to some Material as a component of the recipe.</rdfs:comment>
        <rdfs:label>Method</rdfs:label>
    </owl:Class>
    


    <!-- https://w3id.org/EVI#Reagent -->

    <owl:Class rdf:about="https://w3id.org/EVI#Reagent">
        <rdfs:subClassOf rdf:resource="https://w3id.org/EVI#Material"/>
        <rdfs:comment>A Reagent is a Material used for representing biological objects.</rdfs:comment>
        <rdfs:label>Reagent</rdfs:label>
    </owl:Class>
    


    <!-- https://w3id.org/EVI#Reference -->

    <owl:Class rdf:about="https://w3id.org/EVI#Reference">
        <rdfs:subClassOf rdf:resource="https://w3id.org/EVI#Representation"/>
        <rdfs:comment>A Representation that is used to speify the citation of an EvidenceGraph.</rdfs:comment>
        <rdfs:label>Reference</rdfs:label>
    </owl:Class>
    


    <!-- https://w3id.org/EVI#Representation -->

    <owl:Class rdf:about="https://w3id.org/EVI#Representation">
        <rdfs:subClassOf rdf:resource="https://www.w3.org/ns/prov#Entity"/>
        <rdfs:comment>A Representation is an Entity which represents an instance of EvidenceGraph, an Article, a Claim, a Dataset, a Material, a Method, or a Reference.</rdfs:comment>
        <rdfs:comment>A Representation is an Entity which represents something.</rdfs:comment>
        <rdfs:label>Representation</rdfs:label>
    </owl:Class>
    


    <!-- https://w3id.org/EVI#Service -->

    <owl:Class rdf:about="https://w3id.org/EVI#Service">
        <rdfs:subClassOf rdf:resource="https://w3id.org/EVI#Method"/>
        <rdfs:comment>A Method used during a Computation Activity.</rdfs:comment>
        <rdfs:label>Service</rdfs:label>
    </owl:Class>
    


    <!-- https://w3id.org/EVI#Software -->

    <owl:Class rdf:about="https://w3id.org/EVI#Software">
        <rdfs:subClassOf rdf:resource="https://w3id.org/EVI#Material"/>
        <rdfs:comment>A set of instructions to perform specific Computation Activity.</rdfs:comment>
        <rdfs:label>Software</rdfs:label>
    </owl:Class>
    


    <!-- https://www.w3.org/ns/prov#Activity -->

    <owl:Class rdf:about="https://www.w3.org/ns/prov#Activity">
        <rdfs:comment>An Activity is a process by which an Entity is produced, modified, consumed or used.</rdfs:comment>
        <rdfs:comment>An activity is something that occurs over a period of time and acts upon or with entities; it may include consuming, processing, transforming, modifying, relocating, using, or generating entities.</rdfs:comment>
        <rdfs:label>Activity</rdfs:label>
    </owl:Class>
    


    <!-- https://www.w3.org/ns/prov#Agent -->

    <owl:Class rdf:about="https://www.w3.org/ns/prov#Agent">
        <rdfs:subClassOf rdf:resource="https://www.w3.org/ns/prov#Entity"/>
        <rdfs:comment>An agent is something that bears some form of responsibility for an activity taking place, for the existence of an entity, or for another agent&apos;s activity.</rdfs:comment>
        <rdfs:label>Agent</rdfs:label>
    </owl:Class>
    


    <!-- https://www.w3.org/ns/prov#Entity -->

    <owl:Class rdf:about="https://www.w3.org/ns/prov#Entity">
        <rdfs:comment>An entity is a physical, digital, conceptual, or other kind of thing with some fixed aspects; entities may be real or imaginary.</rdfs:comment>
        <rdfs:comment>Entities are things which may be discussed, real or imaginary.</rdfs:comment>
        <rdfs:label>Entity</rdfs:label>
    </owl:Class>
    


    <!-- https://www.w3.org/ns/prov#Organization -->

    <owl:Class rdf:about="https://www.w3.org/ns/prov#Organization">
        <rdfs:subClassOf rdf:resource="https://www.w3.org/ns/prov#Agent"/>
        <rdfs:comment>An organization is a social or legal institution such as a company, society, etc.</rdfs:comment>
        <rdfs:label>Organization</rdfs:label>
    </owl:Class>
    


    <!-- https://www.w3.org/ns/prov#Person -->

    <owl:Class rdf:about="https://www.w3.org/ns/prov#Person">
        <rdfs:subClassOf rdf:resource="https://www.w3.org/ns/prov#Agent"/>
        <rdfs:comment>Person agents are prople.</rdfs:comment>
        <rdfs:label>Person</rdfs:label>
    </owl:Class>
    


    <!-- 
    ///////////////////////////////////////////////////////////////////////////////////////
    //
    // Rules
    //
    ///////////////////////////////////////////////////////////////////////////////////////
     -->

    <rdf:Description rdf:about="http://purl.org/evi/z">
        <rdf:type rdf:resource="http://www.w3.org/2003/11/swrl#Variable"/>
    </rdf:Description>
    <rdf:Description rdf:about="http://purl.org/evi/a">
        <rdf:type rdf:resource="http://www.w3.org/2003/11/swrl#Variable"/>
    </rdf:Description>
    <rdf:Description rdf:about="http://purl.org/evi/x">
        <rdf:type rdf:resource="http://www.w3.org/2003/11/swrl#Variable"/>
    </rdf:Description>
    <rdf:Description rdf:about="http://purl.org/evi/computation">
        <rdf:type rdf:resource="http://www.w3.org/2003/11/swrl#Variable"/>
    </rdf:Description>
    <rdf:Description rdf:about="http://purl.org/evi/data1">
        <rdf:type rdf:resource="http://www.w3.org/2003/11/swrl#Variable"/>
    </rdf:Description>
    <rdf:Description rdf:about="http://purl.org/evi/data2">
        <rdf:type rdf:resource="http://www.w3.org/2003/11/swrl#Variable"/>
    </rdf:Description>
    <rdf:Description rdf:about="http://purl.org/evi/y">
        <rdf:type rdf:resource="http://www.w3.org/2003/11/swrl#Variable"/>
    </rdf:Description>
    <rdf:Description>
        <swrla:isRuleEnabled rdf:datatype="http://www.w3.org/2001/XMLSchema#boolean">true</swrla:isRuleEnabled>
        <rdfs:comment rdf:datatype="http://www.w3.org/2001/XMLSchema#string"></rdfs:comment>
        <rdfs:label rdf:datatype="http://www.w3.org/2001/XMLSchema#string">S3</rdfs:label>
        <rdf:type rdf:resource="http://www.w3.org/2003/11/swrl#Imp"/>
        <swrl:body>
            <rdf:Description>
                <rdf:type rdf:resource="http://www.w3.org/2003/11/swrl#AtomList"/>
                <rdf:first>
                    <rdf:Description>
                        <rdf:type rdf:resource="http://www.w3.org/2003/11/swrl#IndividualPropertyAtom"/>
                        <swrl:propertyPredicate rdf:resource="https://w3id.org/EVI#derivedFrom"/>
                        <swrl:argument1 rdf:resource="http://purl.org/evi/z"/>
                        <swrl:argument2 rdf:resource="http://purl.org/evi/x"/>
                    </rdf:Description>
                </rdf:first>
                <rdf:rest rdf:resource="http://www.w3.org/1999/02/22-rdf-syntax-ns#nil"/>
            </rdf:Description>
        </swrl:body>
        <swrl:head>
            <rdf:Description>
                <rdf:type rdf:resource="http://www.w3.org/2003/11/swrl#AtomList"/>
                <rdf:first>
                    <rdf:Description>
                        <rdf:type rdf:resource="http://www.w3.org/2003/11/swrl#IndividualPropertyAtom"/>
                        <swrl:propertyPredicate rdf:resource="https://w3id.org/EVI#supports"/>
                        <swrl:argument1 rdf:resource="http://purl.org/evi/x"/>
                        <swrl:argument2 rdf:resource="http://purl.org/evi/z"/>
                    </rdf:Description>
                </rdf:first>
                <rdf:rest rdf:resource="http://www.w3.org/1999/02/22-rdf-syntax-ns#nil"/>
            </rdf:Description>
        </swrl:head>
    </rdf:Description>
    <rdf:Description>
        <swrla:isRuleEnabled rdf:datatype="http://www.w3.org/2001/XMLSchema#boolean">true</swrla:isRuleEnabled>
        <rdfs:comment rdf:datatype="http://www.w3.org/2001/XMLSchema#string"></rdfs:comment>
        <rdfs:label rdf:datatype="http://www.w3.org/2001/XMLSchema#string">S1</rdfs:label>
        <rdf:type rdf:resource="http://www.w3.org/2003/11/swrl#Imp"/>
        <swrl:body>
            <rdf:Description>
                <rdf:type rdf:resource="http://www.w3.org/2003/11/swrl#AtomList"/>
                <rdf:first>
                    <rdf:Description>
                        <rdf:type rdf:resource="http://www.w3.org/2003/11/swrl#IndividualPropertyAtom"/>
                        <swrl:propertyPredicate rdf:resource="https://w3id.org/EVI#usedDataset"/>
                        <swrl:argument1 rdf:resource="http://purl.org/evi/computation"/>
                        <swrl:argument2 rdf:resource="http://purl.org/evi/data1"/>
                    </rdf:Description>
                </rdf:first>
                <rdf:rest>
                    <rdf:Description>
                        <rdf:type rdf:resource="http://www.w3.org/2003/11/swrl#AtomList"/>
                        <rdf:first>
                            <rdf:Description>
                                <rdf:type rdf:resource="http://www.w3.org/2003/11/swrl#IndividualPropertyAtom"/>
                                <swrl:propertyPredicate rdf:resource="https://w3id.org/EVI#generatedBy"/>
                                <swrl:argument1 rdf:resource="http://purl.org/evi/data2"/>
                                <swrl:argument2 rdf:resource="http://purl.org/evi/computation"/>
                            </rdf:Description>
                        </rdf:first>
                        <rdf:rest rdf:resource="http://www.w3.org/1999/02/22-rdf-syntax-ns#nil"/>
                    </rdf:Description>
                </rdf:rest>
            </rdf:Description>
        </swrl:body>
        <swrl:head>
            <rdf:Description>
                <rdf:type rdf:resource="http://www.w3.org/2003/11/swrl#AtomList"/>
                <rdf:first>
                    <rdf:Description>
                        <rdf:type rdf:resource="http://www.w3.org/2003/11/swrl#IndividualPropertyAtom"/>
                        <swrl:propertyPredicate rdf:resource="https://w3id.org/EVI#directlySupports"/>
                        <swrl:argument1 rdf:resource="http://purl.org/evi/data1"/>
                        <swrl:argument2 rdf:resource="http://purl.org/evi/data2"/>
                    </rdf:Description>
                </rdf:first>
                <rdf:rest rdf:resource="http://www.w3.org/1999/02/22-rdf-syntax-ns#nil"/>
            </rdf:Description>
        </swrl:head>
    </rdf:Description>
    <rdf:Description>
        <swrla:isRuleEnabled rdf:datatype="http://www.w3.org/2001/XMLSchema#boolean">true</swrla:isRuleEnabled>
        <rdfs:comment rdf:datatype="http://www.w3.org/2001/XMLSchema#string"></rdfs:comment>
        <rdfs:label rdf:datatype="http://www.w3.org/2001/XMLSchema#string">S4</rdfs:label>
        <rdf:type rdf:resource="http://www.w3.org/2003/11/swrl#Imp"/>
        <swrl:body>
            <rdf:Description>
                <rdf:type rdf:resource="http://www.w3.org/2003/11/swrl#AtomList"/>
                <rdf:first>
                    <rdf:Description>
                        <rdf:type rdf:resource="http://www.w3.org/2003/11/swrl#IndividualPropertyAtom"/>
                        <swrl:propertyPredicate rdf:resource="https://w3id.org/EVI#generatedBy"/>
                        <swrl:argument1 rdf:resource="http://purl.org/evi/z"/>
                        <swrl:argument2 rdf:resource="http://purl.org/evi/y"/>
                    </rdf:Description>
                </rdf:first>
                <rdf:rest rdf:resource="http://www.w3.org/1999/02/22-rdf-syntax-ns#nil"/>
            </rdf:Description>
        </swrl:body>
        <swrl:head>
            <rdf:Description>
                <rdf:type rdf:resource="http://www.w3.org/2003/11/swrl#AtomList"/>
                <rdf:first>
                    <rdf:Description>
                        <rdf:type rdf:resource="http://www.w3.org/2003/11/swrl#IndividualPropertyAtom"/>
                        <swrl:propertyPredicate rdf:resource="https://w3id.org/EVI#supports"/>
                        <swrl:argument1 rdf:resource="http://purl.org/evi/y"/>
                        <swrl:argument2 rdf:resource="http://purl.org/evi/z"/>
                    </rdf:Description>
                </rdf:first>
                <rdf:rest rdf:resource="http://www.w3.org/1999/02/22-rdf-syntax-ns#nil"/>
            </rdf:Description>
        </swrl:head>
    </rdf:Description>
    <rdf:Description>
        <swrla:isRuleEnabled rdf:datatype="http://www.w3.org/2001/XMLSchema#boolean">true</swrla:isRuleEnabled>
        <rdfs:comment rdf:datatype="http://www.w3.org/2001/XMLSchema#string"></rdfs:comment>
        <rdfs:label rdf:datatype="http://www.w3.org/2001/XMLSchema#string">S5</rdfs:label>
        <rdf:type rdf:resource="http://www.w3.org/2003/11/swrl#Imp"/>
        <swrl:body>
            <rdf:Description>
                <rdf:type rdf:resource="http://www.w3.org/2003/11/swrl#AtomList"/>
                <rdf:first>
                    <rdf:Description>
                        <rdf:type rdf:resource="http://www.w3.org/2003/11/swrl#IndividualPropertyAtom"/>
                        <swrl:propertyPredicate rdf:resource="https://w3id.org/EVI#attributedTo"/>
                        <swrl:argument1 rdf:resource="http://purl.org/evi/z"/>
                        <swrl:argument2 rdf:resource="http://purl.org/evi/a"/>
                    </rdf:Description>
                </rdf:first>
                <rdf:rest rdf:resource="http://www.w3.org/1999/02/22-rdf-syntax-ns#nil"/>
            </rdf:Description>
        </swrl:body>
        <swrl:head>
            <rdf:Description>
                <rdf:type rdf:resource="http://www.w3.org/2003/11/swrl#AtomList"/>
                <rdf:first>
                    <rdf:Description>
                        <rdf:type rdf:resource="http://www.w3.org/2003/11/swrl#IndividualPropertyAtom"/>
                        <swrl:propertyPredicate rdf:resource="https://w3id.org/EVI#supports"/>
                        <swrl:argument1 rdf:resource="http://purl.org/evi/a"/>
                        <swrl:argument2 rdf:resource="http://purl.org/evi/z"/>
                    </rdf:Description>
                </rdf:first>
                <rdf:rest rdf:resource="http://www.w3.org/1999/02/22-rdf-syntax-ns#nil"/>
            </rdf:Description>
        </swrl:head>
    </rdf:Description>
    <rdf:Description>
        <swrla:isRuleEnabled rdf:datatype="http://www.w3.org/2001/XMLSchema#boolean">true</swrla:isRuleEnabled>
        <rdfs:comment rdf:datatype="http://www.w3.org/2001/XMLSchema#string"></rdfs:comment>
        <rdfs:label rdf:datatype="http://www.w3.org/2001/XMLSchema#string">S2</rdfs:label>
        <rdf:type rdf:resource="http://www.w3.org/2003/11/swrl#Imp"/>
        <swrl:body>
            <rdf:Description>
                <rdf:type rdf:resource="http://www.w3.org/2003/11/swrl#AtomList"/>
                <rdf:first>
                    <rdf:Description>
                        <rdf:type rdf:resource="http://www.w3.org/2003/11/swrl#IndividualPropertyAtom"/>
                        <swrl:propertyPredicate rdf:resource="https://w3id.org/EVI#derivedFrom"/>
                        <swrl:argument1 rdf:resource="http://purl.org/evi/z"/>
                        <swrl:argument2 rdf:resource="http://purl.org/evi/x"/>
                    </rdf:Description>
                </rdf:first>
                <rdf:rest rdf:resource="http://www.w3.org/1999/02/22-rdf-syntax-ns#nil"/>
            </rdf:Description>
        </swrl:body>
        <swrl:head>
            <rdf:Description>
                <rdf:type rdf:resource="http://www.w3.org/2003/11/swrl#AtomList"/>
                <rdf:first>
                    <rdf:Description>
                        <rdf:type rdf:resource="http://www.w3.org/2003/11/swrl#IndividualPropertyAtom"/>
                        <swrl:propertyPredicate rdf:resource="https://w3id.org/EVI#supports"/>
                        <swrl:argument1 rdf:resource="http://purl.org/evi/x"/>
                        <swrl:argument2 rdf:resource="http://purl.org/evi/z"/>
                    </rdf:Description>
                </rdf:first>
                <rdf:rest rdf:resource="http://www.w3.org/1999/02/22-rdf-syntax-ns#nil"/>
            </rdf:Description>
        </swrl:head>
    </rdf:Description>
</rdf:RDF>



<!-- Generated by the OWL API (version 4.5.9.2019-02-01T07:24:44Z) https://github.com/owlcs/owlapi -->

